TSO.v update

src/tso/TSO.v
@@ -53,3 +53,825 @@ Module TsoMsg.
     left. f_equal; intuition.
   Defined.
 End TsoMsg.
+
+Module TsoMemory.
+  Definition t := list TsoMsg.t.
+
+  Definition empty: t := [].
+  
+  Definition read (loc:Loc.t) (ts:Time.t) (mem:t): option Val.t :=
+    match Time.pred_opt ts with
+      | None => Some Val.default
+      | Some ts => 
+        match List.nth_error mem ts with
+          | None => None
+          | Some msg =>
+            if msg.(TsoMsg.loc) == loc 
+            then Some msg.(TsoMsg.val)
+            else None
+          end
+        end.
+
+  Definition get_msg (ts: Time.t) (mem:t): option TsoMsg.t :=
+      match Time.pred_opt ts with 
+      | None => None
+      | Some ts => List.nth_error mem ts
+      end.
+
+  Definition append (msg: TsoMsg.t) (mem:t): Time.t * t :=
+    (S (length mem), mem ++ [msg]).
+  
+  Definition no_msgs (from to:nat) (pred:TsoMsg.t -> Prop) (mem:t): Prop :=
+    forall ts msg
+    (TS1: from < S ts)
+    (TS2: S ts <= to)
+    (MSG: List.nth_error mem ts = Some msg),
+    ~ pred msg.
+
+  Definition latest (loc:Loc.t) (from to:Time.t) (mem:t): Prop :=
+    TsoMeomory.no_msgs from to (fun msg => msg.(TsoMsg.loc) = loc) mem.
+
+  Fixpoint latest_ts (loc:Loc.t) (from to:Time.t) (mem:t): Prop :=
+    match to with
+    | 0 => 0
+    | S to => 
+      match List.nth_error mem to with
+      | Some (TsoMsg.mk loc0 _ _) =>
+        if (Loc.eq_dec loc0 loc) then S to else latest_ts loc to mem
+      | _ => latest_ts loc to mem
+      end
+    end
+  .
+
+  Definition exclusive (tid:Id.t) (loc:Loc.t) (from to: Time.t) (mem:t):Prop :=
+    TsoMemory.no_msgs from to (fun msg => msg.(TsoMsg.loc) = loc /\ msg.(TsoMsg.tid) <> tid) mem.
+
+  (* Lemmas *)
+
+  Lemma read_mon ts loc val mem1 mem2
+        (READ: TsoMemory.read loc ts mem1 = Some val):
+    TsoMemory.read loc ts (mem1 ++ mem2) = Some val.
+  Proof. Admitted.
+
+  Lemma get_msg_mon ts msg mem1 mem2
+        (READ: TsoMemory.get_msg ts mem1 = Some msg):
+    TsoMemory.get_msg ts (mem1 ++ mem2) = Some msg.
+  Proof. Admitted.
+
+  Lemma get_msg_read ts mem loc val tid
+        (GET: get_msg ts mem = Some (TsoMsg.mk loc val tid)):
+    read loc ts mem = Some val.
+  Proof.
+  Admitted.
+
+  Lemma read_get_msg
+        loc ts mem val
+        (READ: read loc ts mem = Some val):
+    (ts = Time.bot /\ val = Val.default) \/
+    (exists tid, get_msg ts mem = Some (TsoMsg.mk loc val tid)).
+  Proof. Admitted.
+
+  Lemma get_msg_app_inv
+        ts mem1 mem2 m
+        (GET: get_msg ts (mem1 ++ mem2) = Some m):
+    (ts <= length mem1 /\ get_msg ts mem1 = Some m) \/
+    (ts > length mem1 /\ List.nth_error mem2 (ts - (S (length mem1))) = Some m).
+  Proof. Admitted.
+
+  Lemma get_msg_snoc_inv
+        ts mem msg m
+        (GET: get_msg ts (mem ++ [msg]) = Some m):
+    (ts <= length mem /\ get_msg ts mem = Some m) \/
+    (ts = S (length mem) /\ msg = m).
+  Proof. Admitted.
+
+  Lemma get_latest
+        loc mem:
+    exists ts val,
+      (forall ts' val (READ: read loc ts' mem = Some val), ts' <= ts) /\
+      read loc ts mem = Some val.
+  Proof. Admitted.
+
+  Lemma latest_lt
+        loc ts1 ts2 ts3 mem msg
+        (LATEST: TsoMemory.latest loc ts1 ts2 mem)
+        (LT: ts1 < ts3)
+        (MSG: TsoMemory.get_msg ts3 mem = Some msg)
+        (LOC: msg.(TsoMsg.loc) = loc):
+    ts2 < ts3.
+  Proof. Admitted.
+
+  Lemma ge_latest loc ts1 ts2 mem
+        (GE: ts2 <= ts1):
+    TsoMemory.latest loc ts1 ts2 mem.
+  Proof. Admitted.
+
+  Lemma latest_mon1
+        loc ts1 ts2 ts3 mem
+        (LATEST: latest loc ts1 ts3 mem)
+        (LT: ts1 <= ts2):
+    latest loc ts2 ts3 mem.
+  Proof. Admitted.
+
+  Lemma latest_mon2
+        loc ts1 ts2 ts3 mem
+        (LATEST: latest loc ts1 ts3 mem)
+        (LT: ts2 <= ts3):
+    latest loc ts1 ts2 mem.
+  Proof. Admitted.
+
+  Lemma latest_join
+        loc ts ts1 ts2 mem
+        (LATEST1: latest loc ts ts1 mem)
+        (LATEST2: latest loc ts ts2 mem):
+    latest loc ts (join ts1 ts2) mem.
+  Proof. Admitted.
+
+  Lemma latest_ts_spec
+        loc to mem:
+    <<LE: latest_ts loc to mem <= to>> /\
+    <<READ: exists val, read loc (latest_ts loc to mem) mem = Some val>>.
+  Proof. Admitted.
+
+  Lemma latest_ts_mon
+        loc to1 to2 mem
+        (LE: to1 <= to2):
+    latest_ts loc to1 mem <= latest_ts loc to2 mem.
+  Proof. Admitted.
+
+  Lemma latest_ts_append
+        loc to mem1 mem2:
+    latest_ts loc to mem1 <= latest_ts loc to (mem1 ++ mem2).
+  Proof. Admitted.
+
+  Lemma latest_ts_latest
+        loc from to mem
+        (LATEST: latest_ts loc to mem = from):
+    latest loc from to mem.
+  Proof. Admitted.
+
+  Lemma latest_latest_ts
+        loc from to mem
+        (LATEST: latest loc from to mem):
+    latest_ts loc to mem <= from.
+  Proof. Admitted.
+
+  Lemma latest_ts_read_lt
+        loc from to mem v val
+        (LATEST: latest_ts loc to mem = from)
+        (READ: read loc v mem = Some val)
+        (LT: from < v):
+    to < v.
+  Proof. Admitted.
+
+  Lemma latest_ts_read_le
+        loc to mem v val
+        (READ: read loc v mem = Some val)
+        (LE: v <= to):
+    v <= latest_ts loc to mem.
+  Proof. Admitted.
+
+  Lemma no_msgs_split
+        a b c pred mem
+        (AB: a <= b)
+        (BC: b <= c):
+    no_msgs a c pred mem <->
+    no_msgs a b pred mem /\ no_msgs b c pred mem.
+  Proof. Admitted.
+
+  Lemma no_msgs_split'
+        a b c pred mem:
+    no_msgs a b pred mem /\ no_msgs b c pred mem ->
+    no_msgs a c pred mem.
+  Proof. Admitted.
+
+  Lemma no_msgs_full
+        pred from to mem1 mem2
+        (TO: to <= length mem1)
+        (NOMSGS: no_msgs from to pred mem1):
+    no_msgs from to pred (mem1 ++ mem2).
+  Proof. Admitted.
+
+  Lemma no_msgs_weaken
+        a b c pred mem1 mem2
+        (BC: b <= c)
+        (NOMSGS: no_msgs a c pred (mem1 ++ mem2)):
+    no_msgs a b pred mem1.
+  Proof. Admitted.
+
+  Lemma ge_no_msgs
+        ts1 ts2 pred mem
+        (GE: ts2 <= ts1):
+    no_msgs ts1 ts2 pred mem.
+  Proof. Admitted.
+
+  Lemma latest_uniq
+        ts1 ts2 ts loc mem val1 val2
+        (TS1: ts1 <= ts)
+        (TS2: ts2 <= ts)
+        (LATEST1: latest loc ts1 ts mem)
+        (LATEST2: latest loc ts2 ts mem)
+        (MSG1: read loc ts1 mem = Some val1)
+        (MSG2: read loc ts2 mem = Some val2):
+    ts1 = ts2.
+  Proof. Admitted.
+
+End TsoMemory.
+
+Module TsoView.
+Section TsoView.
+  Context `{A: Type, _: orderC A eq}.
+
+  Inductive t := mk {
+    ts: Time.t;
+    annot: A;
+  }.
+  #[local]
+  Hint Constructors t: core.
+
+  Inductive _le (a b:t): Prop :=
+  | _le_intro
+    (TS: le a.(ts) b.(ts))
+    (ANNOT: le a.(annot) b.(annot))
+  .
+
+  Definition _join (a b:t): t :=
+    mk (join a.(ts) b.(ts)) (join a.(annot) b.(annot)).
+
+  Definition _bot: t := mk bot bot.
+
+  Global Program Instance preorder: PreOrder _le.
+  Next Obligation. ii. econs; refl. Qed.
+  Next Obligation. ii. inv H1. inv H2. econs; etrans; eauto. Qed.
+
+  Global Program Instance partialorder: PartialOrder eq _le.
+  Next Obligation.
+    ii. econs.
+    - i. subst. econs; refl.
+    - i. destruct x, x0. inv H1. inv H2. inv H3. ss. f_equal.
+      + intuition.
+      + antisym; ss.
+  Qed.
+
+  Global Program Instance order:
+    @orderC
+      t
+      eq
+      _le
+      _join
+      _bot
+      _ _ _.
+  Next Obligation.
+    unfold _join. destruct a, b; ss. econs; s; apply join_l.
+  Qed.
+  Next Obligation.
+    unfold _join. destruct a, b; ss. econs; s; apply join_r.
+  Qed.
+  Next Obligation.
+    unfold _join. destruct a, b; ss. econs; s; apply join_assoc.
+  Qed.
+  Next Obligation.
+    unfold _join. destruct a, b; ss. econs; s; apply join_comm.
+  Qed.
+  Next Obligation.
+    inv AC. inv BC. econs; s; apply join_spec; ss.
+  Qed.
+  Next Obligation.
+    econs; apply bot_spec.
+  Qed.
+
+  Lemma ts_join a b:
+    (join a b).(TsoView.ts) = join (a.(TsoView,ts)) (b.(TsoView.ts)).
+  Proof. Admitted.
+
+  Lemma ts_ifc a b:
+    (ifc a b).(TsoView.ts) = ifc a b.(TsoView.ts).
+  Proof. Admitted.
+
+  Lemma ts_bot:
+    bot.(TsoView.ts) = bot.
+  Proof. Admitted.
+
+  Lemma eq_time_eq
+        (v1 v2:t)
+        (EQ: v1 = v2):
+    v1.(ts) = v2.(ts).
+  Proof. Admitted.
+
+End TsoView.
+End TsoView.
+
+Module TsoLocal.
+Section TsoLocal.
+  Inductive t := mk {
+    coh: Loc.t -> TsoView.t (A:=unit);
+    vrn: TsoView.t (A:=unit);
+  }.
+  Hint Constructors t.
+
+  Definition read_view (coh:TsoView.t (A:=unit)) (tsx:Time.t): TsoView.t (A:=unit) :=
+    if coh.(TsoView.ts) == tsx
+    then TsoView.mk bot bot
+    else TsoView.mk tsx bot.
+
+  Definition init: t:= mk bot bot.
+
+  Inductive read (vloc res:ValA.t (A:=unit)) (ts:Time.t) (lc1:t) (mem1: TsoMemory.t) (lc2:t): Prop :=
+  | read_intro
+      loc val
+      view_pre view_post
+      (LOC: loc = vloc.(ValA.val))
+      (VIEW_PRE: view_pre = lc1.(vrn))
+      (COH: le (lc1.(coh) loc).(TsoView.ts) ts)
+      (LATEST: TsoMemory.latest loc ts view_pre.(TsoView.ts) mem1)
+      (MSG: TsoMemory.read loc ts mem1 = Some val)
+      (VIEW_POST: view_post = read_view (lc1.(coh) loc) ts)
+      (RES: res = ValA.mk _ val bot)
+      (LC2: lc2 = 
+            mk
+              (fun_add loc (TsoView.mk ts bot) lc1.(coh))
+              (join lc1.(vrn) view_post))
+  .
+  Hint Constructors read.
+
+  Inductive writable (vloc vval:ValA.t (A:=unit)) (tid:Id.t) (lc1:t) (mem1: TsoMemory.t): Prop :=
+    | writable_intro
+        loc cohmax
+        (LOC: loc = vloc.(ValA.val))
+        (COHMAX: fun_max lc1.(coh) cohmax)
+        (EXT: lt cohmax.(TsoView.ts) ts)
+  .
+  Hint Constructors writable.
+
+  Inductive rmw (vloc vold vnew: ValA.t (A:=unit)) (old_ts:Time.t) (ts:Time.t) (tid:Id.t) (lc1:t) (mem1:TsoMemory.t) (lc2:t): Prop:=
+  | rmw_intro
+      loc old new view_post
+      (LOC: loc = vloc.(ValA.val))
+      (COH: le (lc1.(coh) loc).(TsoView.ts) old_ts)
+      (OLD_RANGE: lt old_ts ts)
+      (EX: TsoMemory.exclusive tid loc old_ts ts mem1)
+      (OLD_MSG: TsoMemory.read loc old_ts mem1 = Some old)
+      (OLD: old = vold.(ValA.val))
+      (NEW: new = vnew.(ValA.val))
+      (WRITABLE: writable vloc vnew tid lc1 mem1 ts)
+      (MSG: TsoMemory.get_msg ts mem1 = Some (TsoMsg.mk loc new tid))
+      (VIEW_POST: view_post = TsoView.mk ts bot)
+      (LC2: lc2 = 
+            mk
+              (fun_add loc (TsoView.mk ts bot) lc1.(coh))
+              (join lc1.(vrn) view_post))
+  
+  .
+  Hint Constructors rmw.
+  
+  Inductive rmw_failure (vloc vold res:ValA.t (A:=unit)) (old_ts:Time.t) (lc1:t) (mem1:TsoMemory.t) (lc2:t): Prop :=
+  | rmw_failure_intro
+      loc old
+      view_pre view_post
+      (LOC: loc = vloc.(ValA.val))
+      (VIEW_PRE: view_pre = lc1.(vrn))
+      (COH: le (lc1.(coh) loc).(TsoView.ts) old_ts)
+      (LATEST: TsoMemory.latest loc old_ts view_pre.(TsoView.ts) mem1)
+      (OLD_MSG: TsoMemory.read loc old_ts mem1 = Some old)
+      (OLD: old = vold.(ValA.val))
+      (VIEW_POST: view_post = read_view (lc1.(coh) loc) old_ts)
+      (RES: res = ValA.mk _ old bot)
+      (LC2: lc2 = 
+            mk
+              (fun_add loc (TsoView.mk old_ts bot) lc1.(coh))
+              (join lc1.(vrn) view_post))
+  
+  .
+  Hint Constructors rmw_failure.
+
+  Inductive mfence (lc1 lc2:t): Prop :=
+  | mfence_intro
+      cohmax
+      (COHMAX: fun_max lc1.(coh) cohmax)
+      (LC2: lc2 = 
+            mk
+              lc1.(coh)
+              (join lc1.(vrn) cohmax))
+  .
+  Hint Constructors mfence.
+
+  Inductive write (vloc vval res: ValA.t (A:=unit)) (ts:Time.t) (tid:Id.t) (lc1:t) (mem1: TsoMemory.t) (lc2:t) (mem2:TsoMemory.t): Prop :=
+  | write_intro
+      loc val
+      (LOC: loc = vloc.(ValA.val))
+      (VAL: val = vval.(ValA.val))
+      (RES: res = ValA.mk _ 0 bot)
+      (MEM: TsoMemory.append (TsoMsg.mk loc val tid) mem1 = (ts, mem2))
+      (LC2: lc2 =
+            mk
+              (fun_add loc (TsoView.mk ts bot) lc1.(coh))
+              lc1.(vrn))
+  .
+  Hint Constructors write.
+
+  Inductive step (event:Event.t (A:=unit)) (tid:Id.t) (mem:TsoMemory.t) (lc1 lc2:t): Prop :=
+  | step_internal
+      (EVENT: event = Event.internal)
+      (LC: lc2 = lc1)
+  | step_read
+      vloc res ts ord
+      (EVENT: event = Event.read false false ord vloc res)
+      (STEP: read vloc res ts lc1 mem lc2)
+  | step_rmw
+      vloc vold vnew old_ts ts ordr ordw
+      (EVENT: event = Event.rmw ordr ordw vloc vold vnew)
+      (STEP: rmw vloc vold vnew old_ts ts tid lc1 mem lc2)
+  | step_rmw_failure
+      vloc vold old_ts ord res
+      (EVENT: event = Event.read false true ord vloc res)
+      (STEP: rmw_failure vloc vold res old_ts lc1 mem lc2)
+  | step_mfence
+      b
+      (EVENT: event = Event.barrier b)
+      (BARRIER: Barrier.is_mfence b)
+      (STEP: mfence lc1 lc2)
+  | step_sfence
+      b
+      (EVENT: event = Event.barrier b)
+      (BARRIER: Barrier.is_sfence b)
+      (STEP: sfence lc1 lc2)
+  | step_flush
+      vloc
+      (EVENT: event = Event.flush vloc)
+      (STEP: flush vloc lc1 lc2)ß
+  .
+  Hint Constructors step.
+
+  Inductive view_step (event:Event.t (A:=unit)) (tid:Id.t) (mem1 mem2:TsoMemory.t) (lc1 lc2: t): Prop :=
+  | view_step_internal
+      (EVENT: event = Event.internal)
+      (LC: lc2 = lc1)
+      (MEM: mem2 = mem1)
+  | view_step_read
+      vloc res ts ord
+      (EVENT: event = Event.read false false ord vloc res)
+      (STEP: read vloc res ts lc1 mem1 lc2)
+  | view_step_write
+      vloc vval res ts ord
+      (EVENT: event = Event.write false ord vloc vval res)
+      (STEP: vrmw vloc vold vnew old_ts ts tid lc1 mem1 lc2 mem2)
+  | view_step_rmw
+        vloc vold vnew old_ts ts ordr ordw
+        (EVENT: event = Event.rmw ordr ordw vloc vold vnew)
+        (STEP: vrmw vloc vold vnew old_ts ts tid lc1 mem1 lc2 mem2)
+  | view_step_rmw_failure
+        vloc vold old_ts ord res
+        (EVENT: event = Event.read false true ord vloc res)
+        (STEP: rmw_failure vloc vold res old_ts lc1 mem1 lc2)
+        (MEM: mem2 = mem1)
+  | view_step_mfence
+        b
+        (EVENT: event = Event.barrier b)
+        (BARRIER: Barrier.is_mfence b)
+        (STEP: mfence lc1 lc2)
+        (MEM: mem2 = mem1)
+  | view_step_sfence
+        b
+        (EVENT: event = Event.barrier b)
+        (BARRIER: Barrier.is_sfence b)
+        (STEP: sfence lc1 lc2)
+        (MEM: mem2 = mem1)
+  | view_step_flush
+        vloc
+        (EVENT: event = Event.flush vloc)
+        (STEP: flush vloc lc1 lc2)
+        (MEM: mem2 = mem1)
+  .
+  Hint Constructors view_step.
+
+  Inductive wf_fwdbank (loc:Loc.t) (mem:TsoMemory.t) (coh: Time.t): Prop :=
+  | wf_fwdbank_intro
+      (VAL: exists val, TsoMemory.read loc coh mem = Some val)
+  .
+  Hint Constructors wf_fwdbank.
+
+  Inductive wf_cohmax (lc:t): Prop :=
+  | wf_cohmax_intro
+      cohmax
+      (COHMAX: fun_max lc.(coh) cohmax)
+      (VRN: lc.(vrn).(TsoView.ts) <= cohmax.(TsoView.ts))
+  .
+  Hint Constructors wf_cohmax.
+
+  Inductive wf (tid:Id.t) (mem:TsoMemory.t) (lc:t): Prop :=
+  | wf_intro
+      (COH: forall loc, (lc.(coh) loc).(TsoView.ts) <= List.length mem)
+      (VRN: lc.(vrn).(TsoView.ts) <= List.length mem)
+      (FWDBANK: forall loc, wf_fwd_bank loc mem (lc.(coh) loc).(TsoView.ts))
+      (COHMAX: wf_cohmax lc)
+      (NFWD: forall ts msg
+                (MSG: TsoMemory.get_msg ts mem = Some msg)
+                (TID: msg.(TsoMsg.tid) <> tid),
+            ts <= lc.(vrn).(TsoView.ts))
+      (NINTERVENING: forall loc from to
+                (LATEST: TsoMemory.latest loc from to mem),
+            (lc.(coh) loc).(TsoView.ts) <= from \/ to < (lc.(coh) loc).(TsoView.ts))
+  .
+  Hint Constructors wf.
+
+  (* Lemmas *)
+
+
+
+End TsoLocal.
+End TsoLocal.
+
+Module TsoExecUnit.
+Section TsoExecUnit.
+  Inductive t := mk {
+    state: State.t (A:=unit);
+    local: TsoLocal.t;
+    mem: TsoMemory.t;
+  }.
+  Hint Constructors t.
+
+  Inductive state_step0 (tid:Id.t) (e1 e2: Event.t (A:=unit)) (eu1 eu2:t): Prop :=
+  | state_step0_intro
+      (STATE: State.step e1 eu1.(state) eu2.(state))
+      (LOCAL: TsoLocal.step e2 tid eu1.(mem) eu1.(local) eu2.(local))
+      (MEM: eu2.(mem) = eu1.(mem))
+  .
+  Hint Constructors state_step0.
+
+  Inductive state_step (tid:Id.t) (eu1 eu2:t): Prop :=
+  | state_step_intro
+      e
+      (STEP: state_step0 tid e e eu1 eu2)
+  .
+  Hint Constructors state_step.
+
+  Inductive step (tid:Id.t) (eu1 eu2:t): Prop :=
+  | step_state (STEP: state_step tid eu1 eu2)
+  .
+  Hint Constructors step.
+
+  Inductive view_step0 (tid:Id.t) (e1 e2: Event.t (A:=unit)) (eu1 eu2:t) : Prop :=
+  | view_step0_intro
+      (STATE: State.step e1 eu1.(state) eu2.(state))
+      (LOCAL: TsoLocal.view_step e2 tid eu1.(mem) eu2.(mem) eu1.(local) eu2.(local))
+  .
+  Hint Constructors view_step0.
+
+  Inductive view_step (tid:Id.t) (eu1 eu2:t): Prop :=
+  | view_step_intro
+      e
+      (STEP: view_step0 tid e e eu1 eu2)
+  .
+  Hint Constructors view_step.
+
+  Inductive wf (tid:Id.t) (eu:t): Prop :=
+  | wf_intro
+      (LOCAL: TsoLocal.wf tid eu.(mem) eu.(local))
+  .
+  Hint Constructors wf.
+
+  Inductive le (eu1 eu2:t) : Prop :=
+  | le_intro
+      mem'
+      (LC: TsoLocal.le eu1.(local) eu2.(local))
+      (MEM: eu2.(mem) = eu1.(mem) ++ mem')
+  .
+
+  Global Program Instance le_partial_order: PreOrder le.
+  Next Obligation. 
+      econs.
+      - refl.
+      - rewrite app_nil_r. ss.
+  Qed.
+  Next Obligation.
+      ii. inv H. inv H0. econs; etrans; eauto.
+      rewrite MEM, app_assoc. eauto.
+  Qed.
+
+  (* Lemmas *)
+  Lemma state_step0_wf tid e eu1 eu2
+        (STEP: state_step0 tid e e eu1 eu2)
+        (WF: wf tid eu1):
+      wf tid eu2.
+  Proof. Admitted.
+
+  Lemma state_step_wf tid eu1 eu2
+        (STEP: state_step tid eu1 eu2)
+        (WF: wf tid eu1):
+      wf tid eu2.
+  Proof. Admitted.
+
+  Lemma rtc_state_step_wf tid eu1 eu2
+        (STEP: rtc (state_step tid) eu1 eu2)
+        (WF: wf tid eu1):
+      wf tid eu2.
+  Proof. Admitted.
+
+  Lemma step_wf tid eu1 eu2
+        (STEP: step tid eu1 eu2)
+        (WF: wf tid eu1):
+    wf tid eu2.
+  Proof. Admitted.
+
+  Lemma view_step0_wf tid e eu1 eu2
+        (STEP: view_step0 tid e e eu1 eu2)
+        (WF: wf tid eu1):
+    wf tid eu2.
+  Proof. Admitted.
+
+  Lemma view_step_wf tid eu1 eu2
+        (STEP: view_step tid eu1 eu2)
+        (WF: wf tid eu1):
+    wf tid eu2.
+  Proof. Admitted.
+
+  Lemma rtc_view_step_wf tid eu1 eu2
+        (STEP: rtc (view_step tid) eu1 eu2)
+        (WF: wf tid eu1):
+    wf tid eu2.
+  Proof. Admitted.
+
+  Lemma state_step_incr tid eu1 eu2
+        (STEP: state_step tid eu1 eu2):
+    le eu1 eu2.
+  Proof. Admitted.
+
+  Lemma rtc_state_step_incr tid eu1 eu2
+        (STEP: rtc (state_step tid) eu1 eu2):
+    le eu1 eu2.
+  Proof. Admitted.
+
+  Lemma step_incr tid eu1 eu2
+        (STEP: step tid eu1 eu2):
+    le eu1 eu2.
+  Proof. Admitted.
+
+  Lemma rtc_state_step_mem
+        tid eu1 eu2
+        (STEP: rtc (TsoExecUnit.state_step tid) eu1 eu2):
+      eu1.(TsoExecUnit.mem) = eu2.(TsoExecUnit.mem).
+  Proof. Admitted.
+
+  Lemma no_promise_rmw_spec.
+  Proof. Admitted.
+
+End TsoExecUnit.
+End TsoExecUnit.
+
+Module TsoMachine.
+  Inductive t := mk {
+    tpool: IdMap.t (State.t (A:=unit) * TsoLocal.t);
+    mem: TsoMemory.t;
+  }.
+  Hint Constructors t.
+
+  Definition init (p:program): t := 
+      mk
+        (IndMap.map (fun stmts => (State.init stmts, TsoLocal.init)) p)
+        TsoMemory.empty.
+
+  Inductive is_terminal (m:t) : Prop :=
+  | is_terminal_intro
+      (TERMINAL:
+          forall tid st lc
+            (FIND: IdMap.find tid m.(tpool) = Some (st, lc)),
+            State.is_terminal st)
+  .
+  Hint Constructors is_terminal.
+
+  Inductive step (eustep: forall (tid:Id.t) (eu1 eu2: TsoExecUnit.t), Prop) (m1 m2:t): Prop :=
+  | step_intro
+      tid st1 lc1 st2 lc2
+      (FIND: IdMap.find tid m1.(tpool) = Some (st1, lc1))
+      (STEP: eustep tid (TsoExecUnit.mk st1 lc1 m1.(mem)) (TsoExecUnit.mk st2 lc2 m2.(mem)))
+      (TPOOL: m2.(tpool) = IdMap.add tid (st2, lc2) m1.(tpool))
+  .
+  Hint Constructors step.
+
+  Inductive wf (m:t) : Prop :=
+  | wf_intro
+      (WF: forall tid st lc
+            (FIND: IdMap.find tid m.(tpool) = Some (st, lc)),
+        TsoExecUnit.wf tid (TsoExecUnit.mk st lc m.(mem)))
+  .
+  Hint Constructors wf.
+
+  Inductive exec (p:program) (m:t): Prop :=
+  | exec_intro
+      (STEP: rtc (step TsoExecUnit.step) (init p) m)
+  .
+  Hint Constructors exec.
+
+  Inductive view_exec (p:program) (m:t): Prop :=
+  | view_exec_intro
+      (STEP: rtc (step TsoExecUnit.view_step) (init p) m)
+  .
+  Hint Constructors view_exec.
+
+  Inductive equiv (m1 m2:t) : Prop :=
+  | equiv_intro
+      (TPOOL: IdMap.Equal m1.(tpool) m2.(tpool))
+      (MEM:  m1.(mem) = m2.(mem))
+  .
+
+
+
+  (* Lemmas *)
+
+  Lemma rtc_eu_step_step
+        eustep tid m st1 lc1 mem1 st2 lc2 mem2
+        (FIND: IdMap.find tid m.(tpool) = Some (st1, lc1))
+        (MEM: m.(mem) = mem1)
+        (EX: rtc (eustep tid)
+                 (TsoExecUnit.mk st1 lc1 mem1)
+                 (TsoExecUnit.mk st2 lc2 mem2)):
+    rtc (step eustep)
+      m
+      (mk
+        (IdMap.add tid (st2, lc2) m.(tpool))
+        mem2).
+  Proof. Admitted.
+
+  Lemma init_wf p:
+    wf (init p).
+  Proof. Admitted.
+
+  Lemma step_state_step_wf
+        m1 m2
+        (STEP: step TsoExecUnit.state_step m1 m2)
+        (WF: wf m1):
+    wf m2.
+  Proof. Admitted.
+
+  Lemma rtc_step_state_step_wf
+        m1 m2
+        (STEP: rtc (step TsoExecUnit.state_step) m1 m2)
+        (WF: wf m1):
+    wf m2.
+  Proof. Admitted.
+
+  Lemma step_step_wf
+        m1 m2
+        (STEP: step TsoExecUnit.step m1 m2)
+        (WF: wf m1):
+    wf m2.
+  Proof. Admitted.
+
+  Lemma rtc_step_step_wf
+        m1 m2
+        (STEP: rtc (step TsoExecUnit.step) m1 m2)
+        (WF: wf m1):
+    wf m2.
+  Proof. Admitted.
+
+  Lemma step_view_step_wf
+        m1 m2
+        (STEP: step TsoExecUnit.view_step m1 m2)
+        (WF: wf m1):
+    wf m2.
+  Proof. Admitted.
+
+  Lemma rtc_step_view_step_wf
+        m1 m2
+        (STEP: rtc (step TsoExecUnit.view_step) m1 m2)
+        (WF: wf m1):
+    wf m2.
+  Proof. Admitted.
+
+  Lemma step_mon
+        (eustep1 eustep2: _ -> _ -> _ -> Prop)
+        (EUSTEP: forall tid m1 m2, eustep1 tid m1 m2 -> eustep2 tid m1 m2):
+    forall m1 m2, step eustep1 m1 m2 -> step eustep2 m1 m2.
+  Proof. Admitted.
+
+  Lemma rtc_step_mon
+        (eustep1 eustep2: _ -> _ -> _ -> Prop)
+        (EUSTEP: forall tid m1 m2, eustep1 tid m1 m2 -> eustep2 tid m1 m2):
+    forall m1 m2, rtc (step eustep1) m1 m2 -> rtc (step eustep2) m1 m2.
+  Proof. Admitted.
+
+  Lemma state_exec_wf
+        m1 m2
+        (STEP: state_exec m1 m2)
+        (WF: wf m1):
+    wf m2.
+  Proof. Admitted.
+
+  Lemma unlift_step_state_step
+        m1 m2 tid st1 lc1
+        (STEPS: rtc (step TsoExecUnit.state_step) m1 m2)
+        (TPOOL: IdMap.find tid m1.(tpool) = Some (st1, lc1)):
+    exists st2 lc2,
+      <<TPOOL: IdMap.find tid m2.(tpool) = Some (st2, lc2) /\
+      <<STEPS: rtc (TsoExecUnit.state_step tid)
+                   (TsoExecUnit.mk st1 lc1 m1.(mem))
+                   (TsoExecUnit.mk st2 lc2 m2.(mem))>>.
+  Proof. Admitted.
+
+  Lemma step_get_msg_tpool
+        p m ts msg
+        (STEPS: rtc (step TsoExecUnit.step) (init p) m)
+        (MSG: TsoMemory.get_msg ts m.(mem) = Some msg):
+    exists sl, IdMap.find msg(TsoMsg.tid) m.(tpool) = Some sl.
+  Proof. Admitted.
+End TsoMachine.
